finished monad instance for the identity monad

theories/Ordered4/Monad.v
@@ -9,30 +9,27 @@ Import OTNotations.
  *** The monad typeclass
  ***)
 
-Class MonadOps {MF: forall `(A:OType), Type}
-      {MR: forall `(A:OType), relation (MF A)}
+Class MonadOps (MF: forall `(A:OType), Type)
+      (MR: forall `(A:OType), relation (MF A))
       (M: forall `(A:OType), OType (MF A) (MR A)) : Type :=
   { returnM : forall `{A:OType}, A -o> M A;
     bindM : forall `{A:OType} `{B:OType}, M A -o> (A -o> M B) -o> M B }.
 
 Instance OTHasType_returnM `(MonadOps) `(A:OType) :
-  OTHasType (A -o> M _ _ A) (ot_R _) returnM returnM.
+  OTHasType (A -o> M _ _ A) (OTarrow_R A _) returnM returnM.
 Proof.
   apply OTHasType_Proper. unfold Proper. reflexivity.
 Defined.
 
 Instance OTHasType_bindM `(MonadOps) `(A:OType) `(B:OType) :
-  OTHasType (M _ _ A -o> (A -o> M _ _ B) -o> M _ _ B) (ot_R _) bindM bindM.
+  OTHasType (M _ _ A -o> (A -o> M _ _ B) -o> M _ _ B)
+            (OTarrow_R (M _ _ A) ((A -o> M _ _ B) -o> M _ _ B))
+            bindM bindM.
 Proof.
   apply OTHasType_Proper. unfold Proper. reflexivity.
 Defined.
 
-Typeclasses eauto := debug.
-Definition exM `(MonadOps) `(A:OType) `(B:OType) `(C:OType)
-           m (f: A -o> M _ _ B) (g: B -o> M _ _ C) :=
-  (mkOTerm (A -o> M _ _ C) (fun x => bindM @o@ (f @o@ x) @o@ g)).
-
-Class Monad `{MonadOps} : Prop :=
+Class Monad `(MonadOps) : Prop :=
   {
     monad_return_bind :
       forall `(A:OType) `(B:OType) (f: A -o> M _ _ B) x,
@@ -50,42 +47,23 @@ Class Monad `{MonadOps} : Prop :=
         bindM @o@ m @o@ (mkOTerm _ (fun x => bindM @o@ (f @o@ x) @o@ g));
   }.
 
-
-
 (* Helpful bind notation *)
 Notation "'do' x <- m1 ; m2" :=
-  (bindM m1 (fun x => m2)) (at level 60, right associativity).
-
-
-(***
- *** Automation for monads
- ***)
-
-Instance Proper_returnM `{Monad} `{LR} :
-  Proper (lr_leq ==> lr_leq) returnM.
-Proof. prove_lr_proper. Qed.
-
-Instance Proper_bindM `{Monad} {A B} `{LR A} `{LR B} :
-  Proper (lr_leq ==> lr_leq ==> lr_leq) (bindM : M A -> (A -> M B) -> M B).
-Proof. prove_lr_proper. Qed.
-
-(* Add the monad laws to the LR rewrite set *)
-Hint Rewrite @monad_return_bind @monad_bind_return @monad_assoc : LR.
+  (bindM @o@ m1 (mkOTerm _ (fun x => m2))) (at level 60, right associativity).
 
 
 (***
  *** The Identity Monad
  ***)
 
-Definition Identity (X:Type) := X.
+Definition Identity `(A:OType) : OType (ot_Type A) (ot_R A) := A.
 
-Instance IdMonad_MonadOps : MonadOps Identity :=
-  { returnM := fun A x => x;
-    bindM := fun A B m f => f m;
-    lrM := fun A R => R }.
+Program Instance IdMonad_MonadOps :
+  MonadOps (fun `(A:OType) => T) (fun `(A:OType) => R) (@Identity) :=
+  { returnM := fun `(A:OType) => mkOTerm (A -o> Identity A) (fun x => x);
+    bindM := fun `(A:OType) `(B:OType) => mkOTerm _ (fun m f => f @o@ m) }.
 
-Instance IdMonad : Monad Identity.
-constructor; intros; unfold returnM, bindM, lrM, IdMonad_MonadOps;
-  try assumption; try prove_lr; try prove_lr_proper.
-intros R1 R2 sub; assumption.
+Instance IdMonad : Monad IdMonad_MonadOps.
+Proof.
+  constructor; intros; simpl; reflexivity.
 Qed.
